\documentclass{article}

\usepackage[fleqn]{amsmath}
\usepackage{amsfonts}
\usepackage{amssymb}
\usepackage[margin=1cm]{geometry}

\usepackage{listings}
\usepackage[usenames,dvipsnames,svgnames,table]{xcolor}

\newcommand{\hbind}{>\!\!\!>\!\!\!=}
\newcommand{\happend}{+\!\!\!+}
\newcommand{\ty}{:\!:}
\newcommand{\U}{\bigcup\nolimits}

\makeatletter
\newcommand*\idstyle{%
        \expandafter\id@style\the\lst@token\relax
}
\def\id@style#1#2\relax{%
  \ifcat#1\relax\else
    \ifnum`#1<\uccode`#1%
      \it
    \else
      \ifnum`#1>\uccode`#1%
        \it
      \fi
    \fi
  \fi
}
\makeatother

\lstdefinelanguage{HaskellUlisses} {
	basicstyle=\linespread{1.2}\selectfont\small,
	columns=fullflexible,     %%
	keepspaces=true,          %%
	identifierstyle=\idstyle, %%
	morekeywords={data,class,instance,case,of,where,let,in,do,if,then,else,type,newtype},
	sensitive=true,
	morecomment=[l][\small\it\textbf]{--},
	morecomment=[s][\small\it\textbf]{\{-}{-\}},
	morestring=[b]",
	stringstyle=\texttt,
	showstringspaces=false,
	numberstyle=\tiny,
	numberblanklines=true,
	showspaces=false,
	breaklines=true,
	showtabs=false
}

\lstnewenvironment{code}{\lstset{language=HaskellUlisses,mathescape=true}}{}

\begin{document}
\subsection*{Open Union}
\begin{code}
data $\U_{rs}$ w
data (a :: $* \to *$) $\rhd$ b
instance Functor  $\U_{rs}$ where

class (t :: $* \to *$) $\in$ rs where
instance t $\in$ (t $\rhd$ rs) where
instance t $\in$ rs $\Rightarrow$ t $\in$ (t' $\rhd$ rs) where

inj :: (Functor t, t $\in$ rs) $\Rightarrow$ t v $\to$ $\U_{rs}$ v
prj :: t $\in$ rs $\Rightarrow$ $\U_{rs}$ v $\to$ Maybe (t v)
decomp :: $\U_{t \rhd rs}$ v $\to$ Either ($\U_{rs}$ v) (t v)
\end{code}

\subsection*{Coroutine Data Type}
\begin{code}
data Eff rs a = Eff { runEff :: $\forall$w. (a $\to$ VE rs w) $\to$ VE rs w }
data VE rs w = Val x
                     | E ($\U_{rs}$ (VE rs w))

send :: ($\forall$w. (a $\to$ w) $\to$ $\U_{rs}$ w) $\to$ Eff rs a
send f = Eff ($\lambda$k $\to$ E (f k))

withHandler :: Functor t
                $\Rightarrow$ (a $\to$ Eff rs w)
                $\to$ (t (VE a (t $\rhd$ rs)) $\to$ Eff rs w)
                $\to$ VE a (t $\rhd$ rs)
                $\to$ Eff rs w
withHandler valHandler effHandler (Val x) = valHandler x
withHandler valHandler effHandler (E un) = case decomp un of
    Right tv $\to$ effHandler tv
    Left u $\to$ send ($\lambda$k $\to$ fmap k u) $\hbind$ withHandler valHandler effHandler

-- pure computations
data Void
runPure :: Eff Void a $\to$ a
runPure m = case runEff m Val of
  Val x $\to$ x

-- state
data State s v = GetState (s $\to$ v)
                     | SetState s (() $\to$ v)
runState :: s $\to$ Eff (State s $\rhd$ rs) a $\to$ Eff rs a
runState s m = handleSt (state s) (runEff m Val) where
    handleSt = withHandler return
    state s (GetState k) = handleSt (state s) (k s)
    state s (PutState s$'$ k) = handleSt (state s$'$) (k ())

-- error
data Error e v = Error e
runError :: Eff (Error e $\rhd$ rs) a $\to$ Eff rs (Either e a)
runError m = handleErr (runEff m Val) where
    handleErr = withHandler (return $\circ$ Right) ($\lambda$(Error e) $\to$ return (Left e))
\end{code}
\subsection*{Calculation}
\begin{code}
abc
\end{code}
\subsection*{{\ttfamily ListT} done..}
done wrong:
\begin{code}
newtype ListT m a = ListT { runListT :: m [a] }
wrap a = [a]

instance Monad m $\Rightarrow$ Monad (ListT m) where
    return = ListT $\circ$ return $\circ$ wrap
    (ListT m) $\hbind$ f = ListT (m $\hbind$ mapM (runListT $\circ$ f) $\hbind$ return $\circ$ concat)

instance MonadTrans ListT where
    lift m = ListT (m $\hbind$ return $\circ$ wrap)
\end{code}
monad laws:
\begin{enumerate}
\item $return\: x \hbind f = f\, x$
\begin{code}
   return x $\hbind$ f
-- definition of return
= ListT (return [x]) $\hbind$ f
-- definition of ($\hbind$)
= ListT (return [x] $\hbind$ mapM (runListT $\circ$ f) $\hbind$ return $\circ$ concat)
-- m is a monad
= ListT (mapM (runListT $\circ$ f) [x] $\hbind$ return $\circ$ concat)
-- definition of mapM
= ListT (runListT (f x) $\hbind$ return $\circ$ wrap $\hbind$ return $\circ$ concat)
-- m is a monad
= ListT (runListT (f x) $\hbind$ $\lambda$y $\to$ return (wrap y) $\hbind$ return $\circ$ concat)
= ListT (runListT (f x) $\hbind$ $\lambda$y $\to$ return (concat [y]))
= ListT (runListT (f x) $\hbind$ $\lambda$y $\to$ return y)
= ListT (runListT (f x) $\hbind$ return)
-- m is a monad
= ListT (runListT (f x)))
= f x
\end{code}
\item $m \hbind return = m$
\begin{code}
   m $\hbind$ return
= ListT (runListT m $\hbind$ mapM (runListT $\circ$ (ListT $\circ$ return $\circ$ wrap)) $\hbind$ return $\circ$ concat)
= ListT (runListT m $\hbind$ mapM (return $\circ$ wrap) $\hbind$ return $\circ$ concat)
-- ?mapM_and_concat
= ListT (runListT m $\hbind$ return)
= m

-- ?mapM_and_concat: mapM (return $\circ$ wrap) xs $\hbind$ return $\circ$ concat = return xs
-- base case
   mapM (return $\circ$ wrap) [] $\hbind$ return $\circ$ concat
= return []
-- inductive case
   mapM (return $\circ$ wrap) (x:xs) $\hbind$ return $\circ$ concat
= (return [x] $\hbind$ $\lambda$x$'$ $\to$ mapM (return $\circ$ wrap) xs $\hbind$ $\lambda$xs$'$ $\to$ return (x$'$:xs$'$)) $\hbind$ return $\circ$ concat
= (mapM (return $\circ$ wrap) xs $\hbind$ $\lambda$xs$'$ $\to$ return ([x]:xs$'$)) $\hbind$ return $\circ$ concat
-- m is a monad
= (mapM (return $\circ$ wrap) xs $\hbind$ $\lambda$xs$'$ $\to$ return ([x]:xs$'$)) $\hbind$ return $\circ$ concat
-- m is a monad
= mapM (return $\circ$ wrap) xs $\hbind$ $\lambda$xs$'$ $\to$ return ([x]:xs$'$) $\hbind$ return $\circ$ concat
= mapM (return $\circ$ wrap) xs $\hbind$ $\lambda$xs$'$ $\to$ return (concat ([x]:xs$'$))
= mapM (return $\circ$ wrap) xs $\hbind$ $\lambda$xs$'$ $\to$ return ([x] $\happend$ concat xs$'$)
-- m is a monad
= mapM (return $\circ$ wrap) xs $\hbind$ $\lambda$xs$'$ $\to$ return (concat xs$'$) $\hbind$ $\lambda$ys $\to$ return ([x] $\happend$ ys)
-- m is a monad
= mapM (return $\circ$ wrap) xs $\hbind$ return $\circ$ concat $\hbind$ $\lambda$ys $\to$ return ([x] $\happend$ ys)
-- induction hypothesis
= return xs $\hbind$ $\lambda$ys $\to$ return ([x] $\happend$ ys)
= return ([x] $\happend$ xs)
= return (x:xs)
\end{code}
\item $(m \hbind f) \hbind g) = m \hbind (\lambda x \to f\, x \hbind g)$
\begin{code}
   (m $\hbind$ f) $\hbind$ g
= ListT (runListT m $\hbind$ mapM (runListT $\circ$ f) $\hbind$ return $\circ$ concat) $\hbind$ g
= ListT ((runListT m $\hbind$ mapM (runListT $\circ$ f) $\hbind$ return $\circ$ concat) $\hbind$ mapM (runListT $\circ$ g) $\hbind$ return $\circ$ concat)
= {- TODO -}
= ListT (runListT m $\hbind$ mapM (runListT $\circ$ ($\lambda$x $\to$ f x $\hbind$ g)) $\hbind$ return $\circ$ concat)
= m $\hbind$ $\lambda$x $\to$ f x $\hbind$ g

{- ?lem_if_m_commute1:
       mapM f (xs $\happend$ ys)
    = mapM f xs $\hbind$ $\lambda$xs$'$ $\to$ mapM f ys $\hbind$ $\lambda$ys$'$ $\to$ return (xs$'$ $\happend$ ys$'$)
 -}
-- base case
-- inductive case

{- ?lem_if_m_commute2:
        mapM (runListT $\circ$ f) xs $\hbind$ return $\circ$ concat $\hbind$ mapM (runListT $\circ$ g)
     = mapM (runListT $\circ$ ($\lambda$x $\to$ f x $\hbind$ g)) xs
 -}
-- base case
   mapM (runListT $\circ$ f) [] $\hbind$ return $\circ$ concat $\hbind$ mapM (runListT $\circ$ g)
= return []
= mapM (runListT $\circ$ ($\lambda$x $\to$ f x $\hbind$ g)) xs
-- inductive case
   mapM (runListT $\circ$ f) (x:xs) $\hbind$ return $\circ$ concat $\hbind$ mapM (runListT $\circ$ g)
= (runListT (f x) $\hbind$ $\lambda$x$'$ $\to$ mapM (runListT $\circ$ f) xs $\hbind$ $\lambda$xs$'$ $\to$ return (x$'$:xs$'$)) $\hbind$ return $\circ$ concat $\hbind$ mapM (runListT $\circ$ g)
-- m is a monad
= runListT (f x) $\hbind$ $\lambda$x$'$ $\to$ mapM (runListT $\circ$ f) xs $\hbind$ $\lambda$xs$'$ $\to$ return (x$'$:xs$'$) $\hbind$ return $\circ$ concat $\hbind$ mapM (runListT $\circ$ g)
= runListT (f x) $\hbind$ $\lambda$x$'$ $\to$ mapM (runListT $\circ$ f) xs $\hbind$ $\lambda$xs$'$ $\to$ return (x$'$ $\happend$ concat xs$'$) $\hbind$ mapM (runListT $\circ$ g)
-- m is a monad
= runListT (f x) $\hbind$ $\lambda$x$'$ $\to$ mapM (runListT $\circ$ f) xs $\hbind$ $\lambda$xs$'$ $\to$ return (concat xs$'$) $\hbind$ $\lambda$ys $\to$ return (x$'$ $\happend$ ys) $\hbind$ mapM (runListT $\circ$ g)
= runListT (f x) $\hbind$ $\lambda$x$'$ $\to$ mapM (runListT $\circ$ f) xs $\hbind$ $\lambda$xs$'$ $\to$ return (concat xs$'$) $\hbind$ $\lambda$ys $\to$ mapM (runListT $\circ$ g) (x$'$ $\happend$ ys)
= runListT (f x) $\hbind$ $\lambda$x$'$ $\to$ mapM (runListT $\circ$ f) xs $\hbind$ return $\circ$ concat $\hbind$ $\lambda$ys $\to$ mapM (runListT $\circ$ g) (x$'$ $\happend$ ys)
-- m is commutative
= mapM (runListT $\circ$ f) xs $\hbind$ return $\circ$ concat $\hbind$ $\lambda$ys $\to$ runListT (f x) $\hbind$ $\lambda$x$'$ $\to$ mapM (runListT $\circ$ g) (x$'$ $\happend$ ys)
\end{code}
\end{enumerate}
\end{document}
